More WIP on internal lob

internal/conversion.v
@@ -1,4 +1,3 @@
-(* -*- coq-prog-args: ("-emacs" "-top" "quote_has_type") -*- *)
 (* Runs on top of https://github.com/gmalecha/template-coq *)
 Require Import Template.Template.
 
@@ -10,14 +9,250 @@ Local Open Scope string_scope.
 Local Open Scope positive_scope.
 Local Open Scope list_scope.
 
-Require Export quote_term.
-
 Definition Context := list Ast.term.
 Delimit Scope context_scope with ctx.
 Bind Scope context_scope with Context.
 Notation ε := (@nil Ast.term : Context).
 Definition context_extend (Γ : Context) (x : Ast.term) := cons x Γ.
+Definition context_app (Γ Γ' : Context) := List.app Γ' Γ.
 Notation "Γ ▻ x" := (context_extend Γ x) (at level 55, right associativity).
+Notation "Γ ▻▻ Γ'" := (context_app Γ Γ') (at level 60, right associativity).
+Print Ast.term.
+
+Definition subst_n_name_def
+           (subst_n_name : Ast.term -> Ast.term)
+           (in_term : Ast.def Ast.term)
+: Ast.def Ast.term
+  := match in_term with
+       | {| Ast.dname := dname ; Ast.dtype := dtype ; Ast.dbody := dbody ; Ast.rarg := rarg |}
+         => {| Ast.dname := dname;
+               Ast.dtype := subst_n_name dtype;
+               Ast.dbody := subst_n_name dbody;
+               Ast.rarg := rarg |}
+     end.
+
+Fixpoint subst_n_name (in_term : Ast.term) (subst_term : Ast.term) (var_n : nat) (name : Ast.name) {struct in_term} : Ast.term
+  := match in_term with
+       | Ast.tRel v => match Compare_dec.lt_eq_lt_dec v var_n with
+                         | inleft (left _) => in_term
+                         | inleft (right _) => subst_term
+                         | inright _ => Ast.tRel (pred v)
+                       end
+       | Ast.tVar name0 => match name with
+                             | Ast.nNamed name1
+                               => if String.string_dec name0 name1
+                                  then subst_term
+                                  else in_term
+                             | Ast.nAnon => in_term
+                           end
+       | Ast.tMeta _ => in_term
+       | Ast.tEvar _ => in_term
+       | Ast.tSort _ => in_term
+       | Ast.tCast term0' kind term1'
+         => Ast.tCast (subst_n_name term0' subst_term var_n name)
+                      kind
+                      (subst_n_name term1' subst_term var_n name)
+       | Ast.tProd name' term0' term1'
+         => let new_name := match name, name' with
+                              | Ast.nNamed n0, Ast.nNamed n1
+                                => if String.string_dec n0 n1
+                                   then Ast.nAnon
+                                   else name
+                              | _, _ => name
+                            end in
+            Ast.tProd name'
+                      (subst_n_name term0' subst_term (S var_n) new_name)
+                      (subst_n_name term1' subst_term (S var_n) new_name)
+       | Ast.tLambda name' term0' term1'
+         => let new_name := match name, name' with
+                              | Ast.nNamed n0, Ast.nNamed n1
+                                => if String.string_dec n0 n1
+                                   then Ast.nAnon
+                                   else name
+                              | _, _ => name
+                            end in
+            Ast.tLambda name'
+                        (subst_n_name term0' subst_term (S var_n) new_name)
+                        (subst_n_name term1' subst_term (S var_n) new_name)
+       | Ast.tLetIn name' term0' term1' term2'
+         => let new_name := match name, name' with
+                              | Ast.nNamed n0, Ast.nNamed n1
+                                => if String.string_dec n0 n1
+                                   then Ast.nAnon
+                                   else name
+                              | _, _ => name
+                            end in
+            Ast.tLetIn name'
+                       (subst_n_name term0' subst_term (S var_n) new_name)
+                       (subst_n_name term1' subst_term (S var_n) new_name)
+                       (subst_n_name term2' subst_term (S var_n) new_name)
+       | Ast.tApp f args
+         => Ast.tApp (subst_n_name f subst_term var_n name)
+                     (List.map (fun term' => subst_n_name term' subst_term var_n name) args)
+       | Ast.tConst _ => in_term
+       | Ast.tInd _ => in_term
+       | Ast.tConstruct _ _ => in_term
+       | Ast.tCase n term0' term1' branches
+         => Ast.tCase n
+                      (subst_n_name term0' subst_term var_n name)
+                      (subst_n_name term1' subst_term var_n name)
+                      (List.map (fun term' => subst_n_name term' subst_term var_n name) branches)
+       | Ast.tFix term0' n
+         => Ast.tFix (List.map (subst_n_name_def (fun term' => subst_n_name term' subst_term var_n name)) term0')
+                     n
+       | Ast.tUnknown _ => in_term
+     end.
+
+Fixpoint context_subst_n (in_context : Context) (subst_term : Ast.term) (var_n : nat) (name : Ast.name) {struct in_context} : Context
+  := match in_context with
+       | nil => nil
+       | cons T Ts => context_extend
+                        (context_subst_n Ts subst_term (S var_n) name)
+                        (subst_n_name T subst_term var_n name)
+     end.
+
+(** Quoting the rules from the appendix of the HoTT book *)
+
+Print Ast.term.
+
+Inductive convertible : Context -> Ast.term -> Ast.term -> Ast.term -> Type :=
+with has_type : Context -> Ast.term -> Ast.term -> Type :=
+(**
+<<
+(x₁ : A₁, ..., xₙ : Aₙ) ctx
+-------------------------------- Vble
+x₁ : A₁, ..., xₙ : Aₙ ⊢ xᵢ : Aᵢ
+>> *)
+| has_type_tRel_0 : forall T Γ univ,
+                      has_type Γ T (Ast.tSort univ)
+                      -> has_type (Γ ▻ T) (Ast.tRel 0) T
+| has_type_tRel_S : forall T T' Γ n,
+                      has_type Γ (Ast.tRel n) T
+                      -> has_type (Γ ▻ T') (Ast.tRel (S n)) T.
+
+Class Context_inf := mkContext : Context.
+Definition Let_Context_inf_In (ctx : Context_inf) {T} (f : Context_inf -> T)
+  := f ctx.
+
+(**
+<<
+Γ ⊢ a : A     Γ, x : A, Δ ⊢ b : B
+--------------------------------- Subst₁
+   Γ, Δ[a/x] ⊢ b[a/x] : B[a/x]
+>>
+
+HoTT book says provable by induction.
+*)
+Lemma subst_1 {Γ a A Δ B b}
+: has_type Γ a A -> has_type (Γ ▻ A ▻▻ Δ) b B
+  -> has_type (Γ ▻▻ context_subst_n Δ a (List.length Γ) Ast.nAnon)%list
+              (subst_n_name b a (List.length Γ) Ast.nAnon)
+              (subst_n_name B a (List.length Γ) Ast.nAnon).
+Proof.
+  intros ht1 ht2.
+Admitted.
+
+(**
+
+
+Local Opaque Compare_dec.lt_eq_lt_dec.
+    simpl in *.
+  simpl.
+  induction ht2
+Γ
+Inductive has_type :  Context -> Ast.term -> Ast.term -> Type :=
+| has_type_weaken : forall Γ Γ' T t,
+                      has_type Γ t T
+                      -> has_type (Γ ++ Γ') t T
+| has_type_tRel_0 : forall T Γ,
+                      has_type (Γ ▻ T) (Ast.tRel 0) T
+| has_type_tRel_S : forall T T' Γ n,
+                      has_type Γ (Ast.tRel n) T
+                      -> has_type (Γ ▻ T') (Ast.tRel (S n)) T
+| has_type_tApp : forall Γ A B f x,
+                    has_type Γ f (A ‘→’ B)
+                    -> has_type Γ x A
+                    -> has_type Γ (Ast.tApp f [x]) B
+| has_type_tApp_nil : forall Γ A x,
+                        has_type Γ x A
+                        -> has_type Γ (Ast.tApp x []) A
+| has_type_tApp_split : forall Γ T f x1 x2 xs,
+                          has_type Γ (Ast.tApp (Ast.tApp f [x1]) (cons x2 xs)) T
+                          -> has_type Γ (Ast.tApp f (cons x1 (cons x2 xs))) T
+(* TODO?: Make sure that the beta-expanded term is well-typed? *)
+| has_type_beta_1_type : forall Γ t f T,
+                           has_type Γ t (f (cbv_beta_1 T))
+                           -> has_type Γ t (f T)
+| has_type_eta_1_type : forall Γ t f T,
+                          has_type Γ t (f T)
+                          -> has_type Γ t (f (cbv_beta_1 T))
+| has_type_beta_1_term : forall Γ f t T,
+                           has_type Γ (f (cbv_beta_1 t)) T
+                           -> has_type Γ (f t) T
+| has_type_eta_1_term : forall Γ t f T,
+                          has_type Γ (f t) T
+                          -> has_type Γ (f (cbv_beta_1 t)) T
+(** TODO?: Make sure that the arguments to [sigT] are well-typed? *)
+| has_type_existT
+  : forall Γ A P x y,
+      (*let T := Ast.tApp ‘sigT’ [A; P] in
+    has_type T (Ast.tSort U)
+    -> has_type A (Ast.tSort U1
+    -> has_type P (A ‘→’ Ast.tSort U2)*)
+      has_type Γ x A
+      -> has_type Γ y (Ast.tApp P [x])
+      -> has_type Γ (Ast.tApp ‘existT’ [A; P; x; y]) (Ast.tApp ‘sigT’ [A; P])
+| has_type_qO : forall Γ, has_type Γ qO nat'
+| has_type_qS : forall Γ, has_type Γ qS (nat' ‘→’ nat')
+| has_type_qxI : forall Γ, has_type Γ qxI (positive' ‘→’ positive')
+| has_type_qxO : forall Γ, has_type Γ qxO (positive' ‘→’ positive')
+| has_type_qxH : forall Γ, has_type Γ qxH positive'
+| has_type_qtrue : forall Γ, has_type Γ qtrue bool'
+| has_type_qfalse : forall Γ, has_type Γ qfalse bool'
+| has_type_qAscii : forall Γ, has_type Γ qAscii (bool' ‘→’ bool' ‘→’ bool' ‘→’ bool' ‘→’ bool' ‘→’ bool' ‘→’ bool' ‘→’ bool' ‘→’ ascii')
+| has_type_qEmptyString : forall Γ, has_type Γ qEmptyString string'
+| has_type_qString : forall Γ, has_type Γ qString (ascii' ‘→’ string' ‘→’ string')
+| has_type_qnil : forall Γ T U, has_type Γ T (Ast.tSort U)
+                              -> has_type Γ (Ast.tApp qnil [T]) (Ast.tApp list' [T])
+| has_type_qcons : forall Γ T,
+                     has_type Γ (Ast.tApp qcons [T]) (T ‘→’ Ast.tApp list' [T] ‘→’ Ast.tApp list' [T])
+| has_type_term' : forall Γ, has_type Γ term' (Ast.tSort Ast.sSet)
+| has_type_def' : forall Γ, has_type Γ def' (Ast.tSort Ast.sSet ‘→’ Ast.tSort Ast.sSet)
+| has_type_qmkInd : forall Γ, has_type Γ qmkInd (string' ‘→’ nat' ‘→’ inductive')
+(*| has_type_qstProp : has_type Γ (qtSort ‘’ qsProp) (Ast.tSort (Ast.sType 1))
+| has_type_qstSet : has_type Γ (qtSort ‘’ qsSet) (Ast.tSort (Ast.sType 1))
+| has_type_qstType : forall p p',
+                      denote_positive p = Some p'
+                      -> has_type Γ (qtSort ‘’ (Ast.tApp qsType [p]))
+                                  (Ast.tSort (Ast.sType (1 + p')))*)
+| has_type_qsProp : forall Γ, has_type Γ qsProp sort'
+| has_type_qsSet : forall Γ, has_type Γ qsSet sort'
+| has_type_qsType : forall Γ, has_type Γ qsType (positive' ‘→’ sort')
+| has_type_qnAnon : forall Γ, has_type Γ qnAnon name'
+| has_type_qnNamed : forall Γ, has_type Γ qnNamed (ident' ‘→’ name')
+| has_type_qVmCast : forall Γ, has_type Γ qVmCast cast_kind'
+| has_type_qNativeCast : forall Γ, has_type Γ qNativeCast cast_kind'
+| has_type_qCast : forall Γ, has_type Γ qCast cast_kind'
+| has_type_qRevertCast : forall Γ, has_type Γ qRevertCast cast_kind'
+| has_type_qtRel : forall Γ, has_type Γ qtRel (nat' ‘→’ term')
+| has_type_qtVar : forall Γ, has_type Γ qtVar (ident' ‘→’ term')
+| has_type_qtMeta : forall Γ, has_type Γ qtMeta (nat' ‘→’ term')
+| has_type_qtEvar : forall Γ, has_type Γ qtEvar (nat' ‘→’ term')
+| has_type_qtSort : forall Γ, has_type Γ qtSort (sort' ‘→’ term')
+| has_type_qtCast : forall Γ, has_type Γ qtCast (term' ‘→’ cast_kind' ‘→’ term' ‘→’ term')
+| has_type_qtProd : forall Γ, has_type Γ qtProd (name' ‘→’ term' ‘→’ term' ‘→’ term')
+| has_type_qtLambda : forall Γ, has_type Γ qtLambda (name' ‘→’ term' ‘→’ term' ‘→’ term')
+| has_type_qtLetIn : forall Γ, has_type Γ qtLetIn (name' ‘→’ term' ‘→’ term' ‘→’ term' ‘→’ term')
+| has_type_qtApp : forall Γ, has_type Γ qtApp (term' ‘→’ Ast.tApp list' [term'] ‘→’ term')
+| has_type_qtConst : forall Γ, has_type Γ qtConst (string' ‘→’ term')
+| has_type_qtInd : forall Γ, has_type Γ qtInd (inductive' ‘→’ term')
+| has_type_qtConstruct : forall Γ, has_type Γ qtConstruct (inductive' ‘→’ nat' ‘→’ term')
+| has_type_qtCase : forall Γ, has_type Γ qtCase (nat' ‘→’ term' ‘→’ term' ‘→’ Ast.tApp list' [term'] ‘→’ term')
+| has_type_qtFix : forall Γ, has_type Γ qtFix (mfixpoint' term' ‘→’ nat' ‘→’ term')
+| has_type_qtUnknown : forall Γ, has_type Γ qtUnknown (string' ‘→’ term')
+| has_type_qmkdef : forall Γ T, has_type Γ qmkdef (name' ‘→’ T ‘→’ T ‘→’ nat' ‘→’ Ast.tApp def' [T])
+| has_type_tLambda
+
 
 Local Notation "x ‘→’ y" := (Ast.tProd Ast.nAnon x y) (at level 99, right associativity, y at level 200).
 
