internal/LobsTheoremProof.v
@@ -1,0 +1,309 @@
+Require Import Coq.Setoids.Setoid.
+Require Export Lob.Notations Lob.LobsTheoremStatement.
+
+(** The proof of the theorem *)
+
+Module Type LobExtendedContext <: LobContext.
+  Axiom Preterm : Type.
+  Axiom Context : Type.
+
+  Delimit Scope context_scope with ctx.
+  Bind Scope context_scope with Context.
+
+  Axiom empty_context : Context.
+  Notation ε := empty_context.
+  Axiom context_extend : Context -> Preterm -> Context.
+  Notation "Γ ▻ x" := (context_extend Γ x).
+
+  Delimit Scope preterm_scope with preterm.
+  Bind Scope preterm_scope with Preterm.
+
+  Global Open Scope preterm_scope.
+
+  Axiom box' : Context -> Preterm -> Type.
+
+  Definition box : Preterm -> Type
+    := box' ε.
+
+  Delimit Scope well_typed_term_scope with wtt.
+  Bind Scope well_typed_term_scope with box.
+
+  Notation "□ T" := (box T).
+
+
+  Axiom qbox : Preterm.
+  Notation "‘□’" := qbox.
+
+  Axiom tProd : Preterm -> Preterm -> Preterm.
+  Notation "x ‘→’ y" := (tProd x y) : preterm_scope.
+
+  Axiom tApp : Preterm -> Preterm -> Preterm.
+  Notation "x ‘’ y" := (tApp x y) : preterm_scope.
+
+  Axiom quote : Preterm -> Preterm.
+  Notation "⌜ x ⌝" := (quote x).
+
+
+  Delimit Scope well_typed_term_scope with wtt.
+  Bind Scope well_typed_term_scope with box'.
+End LobExtendedContext.
+
+Module Lob1 (LC : LobExtendedContext) (Import LH : LobHypotheses LC).
+
+  Module Type PreL.
+    Axiom App : forall {A' B' : Preterm},
+                  □ (A' ‘→’ B') -> □ A' -> □ B'.
+
+    Axiom qtProd : Preterm -> Preterm -> Preterm.
+    Notation "x ‘‘→’’ y" := (qtProd x y) : preterm_scope.
+
+    Axiom ttVar0 : forall {Γ T}, box' (Γ ▻ T) T.
+    Notation "‘‘VAR₀’’" := ttVar0.
+
+    Axiom wttLambda_nd : forall {Γ : Context} {B' : Preterm},
+                         forall A' : Preterm, box' (Γ ▻ A') B' -> box' Γ (A' ‘→’ B').
+
+    Axiom wttApp_1_nd : forall {Γ : Context} {A' B' : Preterm},
+                          box' Γ (A' ‘→’ B') -> box' Γ A' -> box' Γ B'.
+
+    Notation "x ‘’ y" := (wttApp_1_nd x%wtt y%wtt) : well_typed_term_scope.
+
+    Axiom box'_weaken : forall {Γ A}, box' ε A -> box' Γ A.
+
+    Notation "‘‘f’’" := (box'_weaken wtt_qf) : well_typed_term_scope.
+  End PreL.
+
+  Module Type L.
+    Include PreL.
+    Axiom L : Preterm.
+    Axiom qL : Preterm.
+    Notation "‘L’" := qL.
+  End L.
+
+  Module Type PostL.
+    Include L.
+
+    Axiom Conv : □ (‘□’ ‘’ ⌜ L ⌝) -> □ (‘□’ ‘’ ‘L’).
+
+    Axiom Conv2 : □ L -> □ (‘□’ ‘’ ‘L’ ‘→’ ‘X’).
+    Axiom Conv2_inv : □ (‘□’ ‘’ ‘L’ ‘→’ ‘X’) -> □ L.
+    Axiom qConv2 : forall {Γ},
+                     box' Γ (‘□’ ‘’ ‘L’) -> box' Γ (‘□’ ‘’ ⌜‘□’ ‘’ ‘L’ ⌝ ‘‘→’’ ‘□’ ‘’ ⌜‘X’ ⌝).
+
+    Axiom Quot : □ L -> □ (‘□’ ‘’ ⌜ L ⌝).
+
+    Axiom qbApp
+    : forall (A' := (‘□’ ‘’ ⌜‘□’ ‘’ ‘L’ ⌝)%preterm)
+             (B' := (‘□’ ‘’ ⌜‘X’ ⌝)%preterm),
+        □ ((A' ‘‘→’’ B') ‘→’ A' ‘→’ B').
+
+    Notation "‘‘App’’" := (box'_weaken qbApp) : well_typed_term_scope.
+
+    (*Axiom qConv
+  : □ (‘□’ ‘’ ⌜‘□’ ‘’ ⌜L ⌝ ⌝ ‘→’ ‘□’ ‘’ ⌜ ‘□’ ‘’ ‘L’ ⌝).
+
+  Notation "‘‘Conv’’" := (box'_weaken qConv) : well_typed_term_scope.*)
+
+    Axiom qQuote
+    : let A := (‘□’ ‘’ ‘L’)%preterm in
+      □ (A ‘→’ (‘□’ ‘’ (⌜ A ⌝))).
+
+    Notation "‘‘Quote’’" := (box'_weaken qQuote) : well_typed_term_scope.
+  End PostL.
+End Lob1.
+
+Module Type Lob1H (LC : LobExtendedContext) (Import LH : LobHypotheses LC).
+  Module Lob1' := Lob1 LC LH.
+  Include Lob1'.PostL.
+End Lob1H.
+
+Module Lob1' (LC : LobExtendedContext) (Import LH : LobHypotheses LC) (Import M : Lob1H LC LH)
+<: LobsTheorem LC LH.
+  Definition lob : X.
+    refine ((fun (ℓ : □ L) => f (App (Conv2 ℓ) (Conv (Quot ℓ))))
+              (Conv2_inv
+                 (wttLambda_nd
+                    (‘□’ ‘’ ‘L’)
+                    (‘‘f’’ ‘’ ((‘‘App’’ ‘’ (qConv2 ‘‘VAR₀’’)) ‘’ ((*‘‘Conv’’ ‘’*) (‘‘Quote’’ ‘’ ‘‘VAR₀’’))))))).
+  Defined.
+End Lob1'.
+
+Module Type PretermPrimitives (Export LC : LobExtendedContext).
+  Axiom tLambda : Preterm -> Preterm -> Preterm.
+  Axiom qtApp : Preterm.
+
+  Notation "‘App’" := qtApp : preterm_scope.
+End PretermPrimitives.
+
+Module Type PretermReflectionPrimitives (Export LC : LobExtendedContext).
+  Axiom qPreterm : Preterm.
+  Notation "‘Preterm’" := qPreterm : preterm_scope.
+End PretermReflectionPrimitives.
+
+Module Type TypingRules (Import LC : LobExtendedContext) (Import PP : PretermPrimitives LC).
+  Axiom capture_avoiding_subst_0 : forall (in_term : Preterm)
+                                          (new_value : Preterm),
+                                     Preterm.
+  Notation "x [ 0 ↦ y ]" := (capture_avoiding_subst_0 x y).
+  Axiom convertible : Context -> Preterm -> Preterm -> Prop.
+  Axiom box'_respectful : forall {Γ A B},
+                            convertible Γ A B
+                            -> box' Γ A
+                            -> box' Γ B.
+  Axiom convertible_refl : forall {Γ}, Reflexive (convertible Γ).
+  Axiom convertible_sym : forall {Γ}, Symmetric (convertible Γ).
+  Axiom convertible_trans : forall {Γ}, Transitive (convertible Γ).
+  Axiom convertible_tApp : forall {Γ A A' B B'},
+                             convertible Γ A A'
+                             -> convertible Γ B B'
+                             -> convertible Γ (tApp A B) (tApp A' B').
+  Axiom convertible_beta_app_lambda
+  : forall Γ A f a,
+      convertible Γ (tApp (tLambda A f) a) (capture_avoiding_subst_0 f a).
+End TypingRules.
+
+Module Lob2 (LC : LobExtendedContext) (Import LH : LobHypotheses LC).
+  Module Lob1' := Lob1 LC LH.
+  Module Type PretermPrimitives' := PretermPrimitives LC.
+  Module Type PretermReflectionPrimitives' := PretermReflectionPrimitives LC.
+  Module Type PreL'.
+    Include Lob1'.PreL.
+    Include PretermPrimitives'.
+    Include PretermReflectionPrimitives'.
+  End PreL'.
+
+  Module L (PL : PreL') <: Lob1'.L.
+    Include PL.
+
+    Definition L0 (h : Preterm) : Preterm
+      := ((‘□’ ‘’ (h ‘’ (quote h))) ‘→’ ‘X’)%preterm.
+
+    Definition qL0 : Preterm.
+    Proof.
+      refine (tLambda
+                ‘Preterm’
+                (‘App’
+                  ‘’ _(*‘□’*)           (*( *)
+             )).
+
+      admit.
+   (*:= (fun h : Preterm => (‘□’ ‘’ (h ‘’ (quote h))) ‘→’ ‘X’).*)
+    Defined.
+
+    Notation "‘L0’" := qL0.
+
+    Definition L : Preterm
+      := L0 ‘L0’.
+
+    Definition qL : Preterm
+      := ‘L0’ ‘’ ⌜ ‘L0’ ⌝.
+
+    Notation "‘L’" := qL.
+  End L.
+
+(*  Module PostL (PL : PreL') (Import TR : TypingRules LC PL) <: Lob1'.PostL.
+    Module L' := L PL.
+    Include L'.
+
+    Definition Conv : □ (‘□’ ‘’ ⌜ L ⌝) -> □ (‘□’ ‘’ ‘L’).
+    Proof.
+      unfold box, L, qL.
+      apply box'_respectful.
+      apply convertible_tApp.
+      { reflexivity. }
+      { unfold L0, qL0.
+        symmetry.
+        etransitivity; [ solve [ apply convertible_beta_app_lambda ] | ].
+        admit. }
+    Defined.
+
+    Axiom Conv2 : □ L -> □ (‘□’ ‘’ ‘L’ ‘→’ ‘X’).
+    Axiom Conv2_inv : □ (‘□’ ‘’ ‘L’ ‘→’ ‘X’) -> □ L.
+    Axiom qConv2 : forall {Γ},
+                     box' Γ (‘□’ ‘’ ‘L’) -> box' Γ (‘□’ ‘’ ⌜‘□’ ‘’ ‘L’ ⌝ ‘‘→’’ ‘□’ ‘’ ⌜‘X’ ⌝).
+
+    Axiom Quot : □ L -> □ (‘□’ ‘’ ⌜ L ⌝).
+
+    Axiom qtApp
+    : forall (A' := (‘□’ ‘’ ⌜‘□’ ‘’ ‘L’ ⌝)%preterm)
+             (B' := (‘□’ ‘’ ⌜‘X’ ⌝)%preterm),
+        □ ((A' ‘‘→’’ B') ‘→’ A' ‘→’ B').
+
+    Notation "‘‘App’’" := (box'_weaken qtApp) : well_typed_term_scope.
+
+    (*Axiom qConv
+  : □ (‘□’ ‘’ ⌜‘□’ ‘’ ⌜L ⌝ ⌝ ‘→’ ‘□’ ‘’ ⌜ ‘□’ ‘’ ‘L’ ⌝).
+
+  Notation "‘‘Conv’’" := (box'_weaken qConv) : well_typed_term_scope.*)
+
+    Axiom qQuote
+    : let A := (‘□’ ‘’ ‘L’)%preterm in
+      □ (A ‘→’ (‘□’ ‘’ (⌜ A ⌝))).
+
+    Notation "‘‘Quote’’" := (box'_weaken qQuote) : well_typed_term_scope.
+
+  End PostL.
+
+
+Module Type Lob2 (LC : LobExtendedContext) (Import LH : LobHypotheses LC).
+  Axiom App : forall {A' B' : Preterm},
+                □ (A' ‘→’ B') -> □ A' -> □ B'.
+
+  Axiom L : Preterm.
+  Axiom qL : Preterm.
+  Notation "‘L’" := qL.
+
+  Axiom qtProd : Preterm -> Preterm -> Preterm.
+  Notation "x ‘‘→’’ y" := (qtProd x y) : preterm_scope.
+
+  Axiom Conv : □ (‘□’ ‘’ ⌜ L ⌝) -> □ (‘□’ ‘’ ‘L’).
+
+  Axiom Conv2 : □ L -> □ (‘□’ ‘’ ‘L’ ‘→’ ‘X’).
+  Axiom Conv2_inv : □ (‘□’ ‘’ ‘L’ ‘→’ ‘X’) -> □ L.
+  Axiom qConv2 : forall {Γ},
+                   box' Γ (‘□’ ‘’ ‘L’) -> box' Γ (‘□’ ‘’ ⌜‘□’ ‘’ ‘L’ ⌝ ‘‘→’’ ‘□’ ‘’ ⌜‘X’ ⌝).
+
+  Axiom Quot : □ L -> □ (‘□’ ‘’ ⌜ L ⌝).
+
+  Axiom wttLambda_nd : forall {Γ : Context} {B' : Preterm},
+                       forall A' : Preterm, box' (Γ ▻ A') B' -> box' Γ (A' ‘→’ B').
+
+  Axiom wttApp_1_nd : forall {Γ : Context} {A' B' : Preterm},
+                        box' Γ (A' ‘→’ B') -> box' Γ A' -> box' Γ B'.
+
+  Notation "x ‘’ y" := (wttApp_1_nd x%wtt y%wtt) : well_typed_term_scope.
+
+  Axiom box'_weaken : forall {Γ A}, box' ε A -> box' Γ A.
+
+  Notation "‘‘f’’" := (box'_weaken wtt_qf) : well_typed_term_scope.
+
+  Axiom qtApp
+  : forall (A' := (‘□’ ‘’ ⌜‘□’ ‘’ ‘L’ ⌝)%preterm)
+           (B' := (‘□’ ‘’ ⌜‘X’ ⌝)%preterm),
+      □ ((A' ‘‘→’’ B') ‘→’ A' ‘→’ B').
+
+  Notation "‘‘App’’" := (box'_weaken qtApp) : well_typed_term_scope.
+
+  Axiom ttVar0 : forall {Γ T}, box' (Γ ▻ T) T.
+
+  Notation "‘‘VAR₀’’" := ttVar0.
+
+  Axiom qQuote
+  : let A := (‘□’ ‘’ ‘L’)%preterm in
+    □ (A ‘→’ (‘□’ ‘’ (⌜ A ⌝))).
+
+  Notation "‘‘Quote’’" := (box'_weaken qQuote) : well_typed_term_scope.
+End Lob1.
+
+Module Lob1' (LC : LobExtendedContext) (Import LH : LobHypotheses LC) (Import M : Lob1 LC LH)
+<: LobsTheorem LC LH.
+  Definition lob : X.
+    refine ((fun (ℓ : □ L) => f (App (Conv2 ℓ) (Conv (Quot ℓ))))
+              (Conv2_inv
+                 (wttLambda_nd
+                    (‘□’ ‘’ ‘L’)
+                    (‘‘f’’ ‘’ ((‘‘App’’ ‘’ (qConv2 ‘‘VAR₀’’)) ‘’ ((*‘‘Conv’’ ‘’*) (‘‘Quote’’ ‘’ ‘‘VAR₀’’))))))).
+  Defined.
+End Lob1'.
+*)
+End Lob2.
