internal/LobsTheoremStatement.v
@@ -1,0 +1,43 @@
+(** The statement of the theorem *)
+Require Export Lob.Notations.
+
+Module Type LobContext.
+  Axiom Preterm : Type.
+
+  Delimit Scope preterm_scope with preterm.
+  Bind Scope preterm_scope with Preterm.
+
+  Axiom box : Preterm -> Type.
+
+  Delimit Scope well_typed_term_scope with wtt.
+  Bind Scope well_typed_term_scope with box.
+
+  Notation "□ T" := (box T) (at level 0).
+
+
+
+  Axiom qbox : Preterm.
+  Notation "‘□’" := qbox.
+
+  Axiom tProd : Preterm -> Preterm -> Preterm.
+  Notation "x ‘→’ y" := (tProd x y) : preterm_scope.
+
+  Axiom tApp : Preterm -> Preterm -> Preterm.
+  Notation "x ‘’ y" := (tApp x y) : preterm_scope.
+
+  Axiom quote : Preterm -> Preterm.
+  Notation "⌜ x ⌝" := (quote x).
+End LobContext.
+
+Module Type LobHypotheses (Export LC : LobContext).
+  Axiom X : Type.
+  Axiom qX : Preterm.
+  Notation "‘X’" := qX : preterm_scope.
+
+  Axiom f : □ ‘X’ -> X.
+  Axiom wtt_qf : □ ((‘□’ ‘’ ⌜ ‘X’ ⌝) ‘→’ ‘X’).
+End LobHypotheses.
+
+Module Type LobsTheorem (LC : LobContext) (Export LH : LobHypotheses LC).
+  Axiom lob : X.
+End LobsTheorem.
